Some code reorganisation and tidying-up

theories/Common/Utils.v
@@ -5,7 +5,11 @@ Require Import Coq.Floats.PrimFloat.
 Require Import Coq.Numbers.BinNums.
 Require Import Coq.Vectors.Vector.
 Require Import Coq.Strings.Ascii.
+From Coq Require Import ssreflect Utf8.
 
+From stdpp Require Import bitvector tactics list.
+
+From SailStdpp Require Import MachineWord.
 
 Import ListNotations.
 
@@ -16,6 +20,72 @@ Local Open Scope string_scope.
 Local Open Scope Z_scope.
 Local Open Scope bool_scope.
 
+Definition eqb {n} (v1 v2 : bv n) : bool :=
+  v1.(bv_unsigned) =? v2.(bv_unsigned).
+Definition ltb {n} (v1 v2 : bv n) : bool :=
+  v1.(bv_unsigned) <? v2.(bv_unsigned).
+Definition leb {n} (v1 v2 : bv n) : bool := 
+  ltb v1 v2 || eqb v1 v2.
+Definition gtb {n} (v1 v2 : bv n) : bool := 
+  ltb v2 v1.
+Definition geb {n} (v1 v2 : bv n) : bool := 
+  gtb v1 v2 || eqb v1 v2.
+
+Local Close Scope Z_scope.
+Local Open Scope bv_scope.
+
+Notation "x =? y" := (eqb x y) (at level 70, no associativity) : bv_scope.
+Notation "x <? y" := (ltb x y) (at level 70, no associativity) : bv_scope.
+Notation "x <=? y" := (leb x y) (at level 70, no associativity) : bv_scope.
+Notation "x >? y" := (gtb x y) (at level 70, no associativity) : bv_scope.
+Notation "x >=? y" := (geb x y) (at level 70, no associativity) : bv_scope.
+
+Local Notation "(<@{ A } )" := (@lt A) (only parsing) : stdpp_scope.
+Local Notation LtDecision A := (RelDecision (<@{A})).
+
+(** Utility converters and lemmas **)
+
+Definition bv_to_Z_unsigned {n} (v : bv n) : Z := v.(bv_unsigned).
+Definition bv_to_N {n}  (v : bv n) : N := Z.to_N v.(bv_unsigned).
+Definition bv_to_bv {n} {m : N} (v : bv n) : (bv m) :=
+  Z_to_bv m (bv_to_Z_unsigned v).
+Definition bv_to_list_bool {n} (v : bv n) : list bool := bv_to_bits v. 
+
+Definition mword_to_bv {n} : mword n -> bv (N.of_nat (Z.to_nat n)) := 
+  fun x => get_word x.
+
+Definition bv_to_mword {n} : bv (N.of_nat (Z.to_nat n)) -> mword n :=
+  match n with
+  | Zneg _ => fun _ => MachineWord.zeros _
+  | Z0 => fun w => w
+  | Zpos _ => fun w => w
+  end.
+Definition bv_to_mword' {n} : bv (N.of_nat (Z.to_nat n)) -> mword n := 
+  fun w => to_word w.
+  
+Definition invert_bits {n} (m : mword n) : (mword n) :=
+  let l : list bool := mword_to_bools m in 
+  let l := map negb l in 
+  let x : mword (Z.of_nat (base.length l)) := of_bools l in
+  let x : Z := int_of_mword false x in 
+  mword_of_int x.
+
+Lemma bv_eqb_eq {n} : forall (a b: bv n), (a =? b) = true <-> a = b.
+Proof.
+  split.
+  - intro H. unfold eqb in H. 
+    apply Z.eqb_eq in H. apply bv_eq in H. exact H.
+  - intro H. rewrite H. unfold eqb. lia.
+Defined.  
+
+Lemma bv1_neqb_eq0 : forall (a : bv 1), (a =? 1%bv) = false <-> a = 0%bv.
+Proof.
+  intros. split.
+  + intro H. unfold eqb in H. apply Z.eqb_neq in H. apply bv_eq.     
+    assert (P: (0 ≤ bv_unsigned a < 2)%Z); [ apply (bv_unsigned_in_range 1 a) |].
+    change (bv_unsigned 0) with 0%Z. change (bv_unsigned 1) with 1%Z in H. lia.
+  + intro H. rewrite H. done.
+Qed.
 
 (** Inlike OCaml version if lists have different sizes, we just terminate
     after consuming the shortest one, without signaling error *)
@@ -77,6 +147,31 @@ Definition bool_bits_of_bytes (bytes : list ascii): list bool
   in
   List.concat (map ascii_to_bits bytes).
 
+Lemma byte_chunks_len {a} (l : list a) l'  :
+  (8 | length l)%nat → 
+  byte_chunks l = Some l' → 
+  length l' = ((length l)/8)%nat.
+Proof.
+  intro Hdiv. unfold Nat.divide in Hdiv. destruct Hdiv as [q Hdiv].
+
+  assert (P: ∀ q (l : list a) l', length l = (q*8)%nat → byte_chunks l = Some l' → length l' = q).
+  { intro q'. induction q' as [| n IH].
+    { intros l0 l0' Hlen Hbytes. simpl in Hlen. apply nil_length_inv in Hlen. subst.
+      simpl in Hbytes. injection Hbytes. intros. subst. done. }
+    { intros l0 l0' Hlen Hbytes. unfold byte_chunks in Hbytes.
+      destruct l0 eqn:E; [ done |].
+      repeat case_match; try done. 
+      assert (Hlensub: length l8 = (n*8)%nat).
+      { repeat rewrite cons_length in Hlen. simpl in Hlen. lia. }
+        specialize IH with (l:=l8) (l':=l9). 
+        apply IH in Hlensub; [| done]. 
+        injection Hbytes. intro H'.
+        rewrite <- H'. rewrite cons_length. lia. } }
+  
+  intro Hbytes. specialize P with (l:=l). apply P; try done.
+  rewrite Hdiv. rewrite Nat.div_mul; lia.    
+  Qed.
+
 (* could be generalized as monadic map, or implemented as composition
    of [map] and [sequence]. *)
 Fixpoint try_map {A B:Type} (f : A -> option B) (l:list A) : option (list B)
@@ -93,6 +188,82 @@ Fixpoint try_map {A B:Type} (f : A -> option B) (l:list A) : option (list B)
       | None => None
       end
   end.
+
+  Fact try_map_length
+  {A B:Type}
+  (f : A -> option B) (l:list A)
+  (l':list B):
+  try_map f l = Some l' -> length l = length l'.
+Proof.
+  intros H.
+  revert l' H.
+  induction l.
+  - intros l' H.
+    cbn in *.
+    inversion H.
+    reflexivity.
+  - intros l' H.
+    cbn in *.
+    destruct (f a) eqn:Hfa; [| inversion H].
+    destruct (try_map f l) eqn:Htry; [| inversion H].
+    destruct l' as [| l0' l']; inversion H.
+    subst.
+    cbn.
+    f_equal.
+    apply IHl.
+    reflexivity.
+Qed.
+
+Lemma try_map_to_map {A B:Type} (f : A -> option B) (l : list A) (l' : list B) : 
+  try_map f l = Some l' ↔  
+  map f l = map Some l'.
+Proof. 
+  revert l l'. 
+  assert (H: ∀ n l l', length l = n → try_map f l = Some l' ↔ map f l = map Some l').
+  { induction n as [| m IH].
+    + intros l l' H_len. apply list.nil_length_inv in H_len. 
+      subst. simpl. split; intro H. 
+      - inversion H. subst. reflexivity.
+      - symmetry in H. apply map_eq_nil in H. subst. reflexivity. 
+    + intros l l' H_len. destruct l as [| h t ] eqn:H_l; [ done |].
+      split; intro H; rewrite list.cons_length in H_len; apply eq_add_S in H_len.
+      - simpl in H. case_match eqn:H_h; try done. case_match eqn:H_t; try done.
+        match goal with 
+        | _: try_map _ ?t = Some ?l
+          |- _ 
+            => apply (IH t l H_len) in H_t
+        end.    
+        simpl. inversion H as [H']. 
+        rewrite H_h H_t. reflexivity.
+      - simpl. simpl in H. 
+        assert (H_len': length l' = S m). 
+        { rewrite <- (map_length f) in H_len. rewrite <- H_len. 
+          rewrite <- (cons_length (f h)). rewrite H. by rewrite map_length. }          
+        destruct l' as [|h' t'] eqn:H_l'; [ done |].   
+        case_match eqn:H_h; try done. case_match eqn:H_t. 
+        * apply f_equal. subst. 
+          apply (IH t) in H_t; try done. rewrite H_t in H. rewrite <- map_cons in H.
+          by simplify_list_eq. 
+        * subst. simpl in H. 
+          apply (app_inj_2 [Some b] [Some h']) in H;
+          [| rewrite !map_length; rewrite cons_length in H_len'; lia ].  
+          destruct H as [_ H].
+          apply (IH t) in H; [| reflexivity ]. rewrite H in H_t. done.  
+  } 
+  intros l l'. by apply (H (length l) l l').
+Qed.
+
+Lemma try_map_app {A B:Type} (f : A -> option B) (l1 l2 : list A) (l1' l2' : list B) : 
+  try_map f (l1++l2)%list = Some (l1'++l2')%list →  
+  length l1 = length l1' → 
+  try_map f l1 = Some l1' ∧ try_map f l2 = Some l2'.
+Proof.
+  intros H_map H_len.
+  apply try_map_to_map in H_map. rewrite !map_app in H_map.
+  apply (list.app_inj_1) in H_map; [| by rewrite !map_length ]. 
+  destruct H_map as [? ?].
+  split; by apply try_map_to_map.
+Qed.
 
 Definition Z_integerRem_t := Z.rem.
 
@@ -132,10 +303,8 @@ Lemma string_eq_refl: forall x : string, String.compare x x = Eq.
 Proof.
   intros x.
   induction x.
-  -
-    auto.
-  -
-    cbn.
+  - auto.
+  - cbn.
     rewrite ascii_eq_refl.
     assumption.
 Qed.
@@ -147,6 +316,6 @@ Lemma string_eq_trans: forall x y z : string,
 Proof.
   intros x y z H0 H1.
   apply String.compare_eq_iff in H0, H1.
-  rewrite H0, H1.
+  rewrite H0 H1.
   apply string_eq_refl.
 Qed.
